q3

A1/Q3.dfy
@@ -1,59 +1,9 @@
-/*
-Explanation:
-We see that number of tuple that can add up to sum, following the pattern
-0,1,2,3,4,5,6,7,8,...,n
-There are 1 tuple that can adds up to 0 (0,0)
-There are 2 tuple that can adds up to 1 (0,1),(1,0)
-There are 3 tuple that can adds up to 2 (0,2),(1,1),(2,0)
-There are 4 tuple that can adds up to 3 (0,3),(1,2),(2,1),(3,0)
-
-A tuple (x,y) can be computed given i
-By iteratively subtracting i with the sum_of_index (sum_of_index = 0 + 1 + 2 + ...)
-Increment the current index during every iteration 
-
-Stop it when i - (sum_of_index + next_index) < 0
-Then we can find x and y using equations below
-x = i - sum_of_index
-y = next_index - x - 1;
-Because at this point, sum_of_index is now equal to the lowest index at the given sum
-For example,
-Index = 8,
-sum_of_index = 0 + 1 + 2 + 3 = 6, as i - sum_of_index would then become nagative if we include 4
-sum_of_index = 6 which is the lowest starting point for sum 3
-x = 8 - 6 = 2
-y = 4 - 2 - 1 = 1
-(2, 1)
-
-Sum     Index   Tuple
-0		0 		0,0
-1		1		0,1
-1		2		1,0
-2		3		0,2
-2		4		1,1
-2		5		2,0
-3		6		0,3
-3		7		1,2
-3		8		2,1
-3		9		3,0
-*/
-function method findXY(sum : nat, next: nat, i : nat): (nat, nat)
-requires i >= 0;
-requires sum >= 0 && sum <= i;
-requires next >= 0;
-decreases i - sum - next
-ensures sum <= i;
-{
-    //var x := i - sum;
-    //var y := next - x - 1;
-    if (sum + next <= i) then findXY(sum + next, next + 1, i) else (i - sum, next - (i - sum) - 1)
-}
-
 function method unpair (i: nat ): (nat, nat)
 requires i >= 0;
-{ // TODO 
-    var (x, y) := findXY(0, 0, i);
-    var part := (x,y);
-    part
+decreases i;
+{ 
+    if (i == 0) then (0, 0) else var (p, q) := unpair(i - 1); 
+    if (q > 0) then (p + 1, q - 1) else (q, p + 1)
 }
 
 function method pick (i: nat ): nat
@@ -62,20 +12,32 @@ function method pick (i: nat ): nat
     x + i * y
 }
 
-function method findFinalIndex(a: nat , b: nat ): nat
+function method reverse (x: nat, y: nat): nat
+    decreases x
 {
-    ((a + b) * (a + b + 1)) / 2 + a
+    if (x == 0 && y == 0) then 0 else
+        if (x > 0 && y >= 0) then 1 + reverse(x - 1, y + 1) else
+            if (x == 0 && y > 0) then 1 + reverse(y - 1, x) else 
+                0
+}
+
+
+lemma check(a: nat , b: nat, i: nat)
+    requires a >= 0;
+    requires b >= 0;
+    ensures exists x,y :: i == reverse(x, y) == reverse(a, b) ==> x == unpair(i).0 && y == unpair(i).1;
+{
+
 }
 
 method catchTheSpy (a: nat , b: nat )
-requires findFinalIndex(a,b) >= 0;
-requires a + findFinalIndex(a,b) * b == pick(findFinalIndex(a,b));
 {
     var i := 0;
     while a + i * b != pick (i)
-    invariant findFinalIndex(a, b) >= i;
-    decreases findFinalIndex(a, b) - i; 
+    invariant reverse(a, b) >= 0;
+    decreases reverse(a, b) - i; 
     { 
+        check(a, b, i);
         i := i + 1; 
     }
 }
